src/protocol/DNS.Protocol.Parser.EverParseAdapter.fst
@@ -12,7 +12,12 @@ let generated_dns_header_validator_linked : bool = true
 
 let generated_dns_root_question_validator_linked : bool = true
 
+let generated_dns_single_label_question_validator_linked : bool = true
+
 let generated_dns_header_validator = DNSProtocol.validate__dns_header
 
 let generated_dns_root_question_validator =
   DNSProtocol.validate__dns_root_question
+
+let generated_dns_single_label_question_validator label_length =
+  DNSProtocol.validate__dns_single_label_question label_length
